WIP generalize model to not-quite-floats

theories/MaxOfTwoNumbers/Model.v
@@ -48,32 +48,42 @@ Definition W_U : tensor _ _ := Eval cbv in tensor_of_list MaxOfTwoNumbers.Parame
 Definition b_U : tensor _ _ := Eval cbv in tensor_of_list MaxOfTwoNumbers.Parameters.b_U.
 
 #[local] Notation FLOAT := float (only parsing). (* or Q *)
-
 Section with_batch.
   Context {r} {batch : Shape r} {pos}
     (s := (batch ::' pos)%shape)
-    (resid_shape := (s ::' cfg.d_model)%shape).
+    (resid_shape := (s ::' cfg.d_model)%shape)
+    {A} {coer_float : has_coer float A} {coerZ : has_coer Z A}
+    {zeroA : has_zero A}
+    {addA : has_add A} {subA : has_sub A} {mulA : has_mul A} {divA : has_div A}
+    {sqrtA : has_sqrt A} {expA : has_exp A}.
 
-  Definition embed (tokens : tensor s IndexType) : tensor resid_shape FLOAT
-    := HookedTransformer.embed W_E tokens.
+  #[local] Set Warnings Append "-uniform-inheritance,-ambiguous-paths".
+  #[local] Coercion coer_tensor_float {r s} (x : @tensor r s float) : @tensor r s A
+    := Tensor.map coer x.
+  #[local] Set Warnings Append "uniform-inheritance,ambiguous-paths".
+  #[local] Coercion coerA' (x : float) : A := coer x.
 
-  Definition pos_embed (tokens : tensor s IndexType) : tensor resid_shape FLOAT
-    := HookedTransformer.pos_embed (n_ctx:=cfg.n_ctx) W_pos tokens.
+  Definition embed (tokens : tensor s IndexType) : tensor resid_shape A
+    := HookedTransformer.embed (A:=A) W_E tokens.
 
-  Definition ln_final (resid : tensor resid_shape FLOAT) : tensor resid_shape FLOAT
-    := HookedTransformer.ln_final cfg.eps ln_final_w ln_final_b resid.
+  Definition pos_embed (tokens : tensor s IndexType) : tensor resid_shape A
+    := HookedTransformer.pos_embed (A:=A) (n_ctx:=cfg.n_ctx) W_pos tokens.
 
-  Definition unembed (resid : tensor resid_shape FLOAT) : tensor (s ::' cfg.d_vocab_out) FLOAT
-    := HookedTransformer.unembed W_U b_U resid.
+  Definition ln_final (resid : tensor resid_shape A) : tensor resid_shape A
+    := HookedTransformer.ln_final (A:=A) cfg.eps ln_final_w ln_final_b resid.
+
+  Definition unembed (resid : tensor resid_shape A) : tensor (s ::' cfg.d_vocab_out) A
+    := HookedTransformer.unembed (A:=A) W_U b_U resid.
 
   Definition blocks_params : list _
-    := [(L0_attn_W_Q, L0_attn_W_K, L0_attn_W_V, L0_attn_W_O,
-          L0_attn_b_Q, L0_attn_b_K, L0_attn_b_V,
-          L0_attn_b_O,
-          L0_ln1_w, L0_ln1_b)].
+    := [(L0_attn_W_Q:tensor _ A, L0_attn_W_K:tensor _ A, L0_attn_W_V:tensor _ A, L0_attn_W_O:tensor _ A,
+          L0_attn_b_Q:tensor _ A, L0_attn_b_K:tensor _ A, L0_attn_b_V:tensor _ A,
+          L0_attn_b_O:tensor _ A,
+          L0_ln1_w:tensor _ A, L0_ln1_b:tensor _ A)].
 
-  Definition logits (tokens : tensor s IndexType) : tensor (s ::' cfg.d_vocab_out) FLOAT
+  Definition logits (tokens : tensor s IndexType) : tensor (s ::' cfg.d_vocab_out) A
     := HookedTransformer.logits
+         (A:=A)
          (n_ctx:=cfg.n_ctx)
          cfg.eps
          W_E
@@ -89,7 +99,7 @@ Section with_batch.
 
   (** convenience *)
   Definition masked_attn_scores (tokens : tensor s IndexType)
-    : tensor (batch ::' cfg.n_heads ::' pos ::' pos) FLOAT
+    : tensor (batch ::' cfg.n_heads ::' pos ::' pos) A
     := Option.invert_Some
          (HookedTransformer.HookedTransformer.masked_attn_scores
             (n_ctx:=cfg.n_ctx)
@@ -104,7 +114,7 @@ Section with_batch.
             tokens).
 
   Definition attn_pattern (tokens : tensor s IndexType)
-    : tensor (batch ::' cfg.n_heads ::' pos ::' pos) FLOAT
+    : tensor (batch ::' cfg.n_heads ::' pos ::' pos) A
     := Option.invert_Some
          (HookedTransformer.HookedTransformer.attn_pattern
             (n_ctx:=cfg.n_ctx)
@@ -122,10 +132,10 @@ End with_batch.
 Notation model := logits (only parsing).
 
 Definition loss_fn {r} {batch : Shape r} {return_per_token : with_default "return_per_token" bool false}
-  (logits : tensor (batch ::' cfg.n_ctx ::' cfg.d_vocab_out) FLOAT)
+  (logits : tensor (batch ::' cfg.n_ctx ::' cfg.d_vocab_out) A)
   (tokens : tensor (batch ::' cfg.n_ctx) IndexType)
-  : tensor (if return_per_token return Shape (if return_per_token then _ else _) then Shape.squeeze batch else []) FLOAT
-  := (let logits : tensor (batch ::' _) FLOAT
+  : tensor (if return_per_token return Shape (if return_per_token then _ else _) then Shape.squeeze batch else []) A
+  := (let logits : tensor (batch ::' _) A
         := PArray.checkpoint (logits.[…, -1, :]) in
       let true_maximum : tensor (batch ::' 1) IndexType
         := reduce_axis_m1 (keepdim:=true) Reduction.max tokens in
@@ -133,23 +143,23 @@ Definition loss_fn {r} {batch : Shape r} {return_per_token : with_default "retur
         := log_softmax_dim_m1 logits in
       let correct_log_probs
         := PArray.checkpoint (gather_dim_m1 log_probs true_maximum) in
-      if return_per_token return (tensor (if return_per_token return Shape (if return_per_token then _ else _) then _ else _) FLOAT)
+      if return_per_token return (tensor (if return_per_token return Shape (if return_per_token then _ else _) then _ else _) A)
       then -Tensor.squeeze correct_log_probs
       else -Tensor.mean correct_log_probs)%core.
 
 Definition acc_fn {r} {batch : Shape r} {return_per_token : with_default "return_per_token" bool false}
-  (logits : tensor (batch ::' cfg.n_ctx ::' cfg.d_vocab_out) FLOAT)
+  (logits : tensor (batch ::' cfg.n_ctx ::' cfg.d_vocab_out) A)
   (tokens : tensor (batch ::' cfg.n_ctx) IndexType)
-  : tensor (if return_per_token return Shape (if return_per_token then _ else _) then batch else []) FLOAT
-  := (let pred_logits : tensor (batch ::' _) FLOAT
+  : tensor (if return_per_token return Shape (if return_per_token then _ else _) then batch else []) A
+  := (let pred_logits : tensor (batch ::' _) A
         := PArray.checkpoint (logits.[…, -1, :]) in
       let pred_tokens : tensor batch IndexType
         := reduce_axis_m1 (keepdim:=false) Reduction.argmax pred_logits in
       let true_maximum : tensor batch IndexType
         := reduce_axis_m1 (keepdim:=false) Reduction.max tokens in
-      let res : tensor _ FLOAT
+      let res : tensor _ A
         := PArray.checkpoint (Tensor.of_bool (Tensor.map2 eqb pred_tokens true_maximum)) in
-      if return_per_token return (tensor (if return_per_token return Shape (if return_per_token then _ else _) then _ else _) FLOAT)
+      if return_per_token return (tensor (if return_per_token return Shape (if return_per_token then _ else _) then _ else _) A)
       then res
       else Tensor.mean res)%core.
 
