theories/TransformerLens/HookedTransformer/Instances.v
@@ -33,8 +33,8 @@ Module HookedTransformer.
               => apply (Tensor.of_bool_Proper_dep _ _ R)
             | [ |- ?R (Tensor.map2 _ _ _ _) (Tensor.map2 _ _ _ _) ]
               => apply (Tensor.map2_Proper_dep _ _ R)
-           | [ |- ?R (Tensor.map2' _ _ _ _) (Tensor.map2' _ _ _ _) ]
-             => apply (Tensor.map2'_Proper_dep _ _ R _ _ R)
+            | [ |- ?R (Tensor.map2' _ _ _ _) (Tensor.map2' _ _ _ _) ]
+              => apply (Tensor.map2'_Proper_dep _ _ R _ _ R)
             | [ |- ?R (Tensor.map _ _ _) (Tensor.map _ _ _) ]
               => apply (Tensor.map_Proper_dep _ _ R)
             | [ |- ?R (Tensor.map' _ _ _) (Tensor.map' _ _ _) ]
@@ -55,8 +55,8 @@ Module HookedTransformer.
               => apply (Tensor.where__Proper_dep _ _ R)
             | [ |- ?R (Tensor.repeat _ _ _) (Tensor.repeat _ _ _) ]
               => apply (Tensor.repeat_Proper_dep _ _ R)
-           | [ |- ?R (Tensor.broadcast _ _) (Tensor.broadcast _ _) ]
-             => apply (Tensor.broadcast_Proper_dep _ _ R)
+            | [ |- ?R (Tensor.broadcast _ _) (Tensor.broadcast _ _) ]
+              => apply (Tensor.broadcast_Proper_dep _ _ R)
             | [ |- ?R (@SliceIndex.slice ?A ?ri ?ro ?idxs ?s _ _) (@SliceIndex.slice ?A ?ri ?ro ?idxs ?s _ _) ]
               => eapply (@SliceIndex.slice_Proper A ri ro idxs s R)
             | [ |- ?R (@FancyIndex.slice ?rb ?sb ?ri ?ro ?s ?A ?idxs _ _) (@FancyIndex.slice ?rb ?sb ?ri ?ro ?s ?A' ?idxs' _ _) ]
@@ -245,7 +245,6 @@ Module HookedTransformer.
              ==> Dependent.idR
              ==> (Dependent.const eq ==> Dependent.idR)
              ==> Dependent.idR
-             ==> Dependent.idR
              ==> Tensor.eqfR ==> Tensor.eqfR ==> Tensor.eqfR ==> Tensor.eqfR)
           (@forward r s d_model).
     Proof. cbv [forward]; t. Qed.
@@ -270,10 +269,10 @@ Module HookedTransformer.
 
     #[export] Instance q_Proper_dep {r batch pos n_heads d_model d_head use_split_qkv_input}
       : Dependent.Proper
-          ((Dependent.idR ==> Dependent.idR ==> Dependent.idR)
-             ==> Dependent.idR
+          ((Dependent.const eq ==> Dependent.idR)
              ==> (Dependent.idR ==> Dependent.idR ==> Dependent.idR)
              ==> Dependent.idR
+             ==> (Dependent.idR ==> Dependent.idR ==> Dependent.idR)
              ==> Tensor.eqfR
              ==> Tensor.eqfR
              ==> Tensor.eqfR
@@ -281,33 +280,33 @@ Module HookedTransformer.
           (@q r batch pos n_heads d_model d_head use_split_qkv_input).
     Proof. cbv [q]; repeat first [ t_step | apply einsum_input_Proper_dep ]. Qed.
 
-    #[export] Instance q_Proper {A r batch addA zeroA mulA defaultA pos n_heads d_model d_head use_split_qkv_input W_Q b_Q}
-      : Proper (Tensor.eqf ==> Tensor.eqf) (@q A r batch addA zeroA mulA defaultA pos n_heads d_model d_head use_split_qkv_input W_Q b_Q).
+    #[export] Instance q_Proper {A r batch pos n_heads d_model d_head use_split_qkv_input coerZ addA zeroA mulA W_Q b_Q}
+      : Proper (Tensor.eqf ==> Tensor.eqf) (@q A r batch pos n_heads d_model d_head use_split_qkv_input coerZ addA zeroA mulA W_Q b_Q).
     Proof. apply q_Proper_dep; repeat intro; subst; reflexivity. Qed.
 
     #[export] Instance k_Proper_dep {r batch pos n_heads d_model d_head use_split_qkv_input}
-  : Dependent.Proper
-      ((Dependent.idR ==> Dependent.idR ==> Dependent.idR)
-         ==> Dependent.idR
-         ==> (Dependent.idR ==> Dependent.idR ==> Dependent.idR)
-         ==> Dependent.idR
-         ==> Tensor.eqfR
-         ==> Tensor.eqfR
-         ==> Tensor.eqfR
-         ==> Tensor.eqfR)
-      (@k r batch pos n_heads d_model d_head use_split_qkv_input).
+      : Dependent.Proper
+          ((Dependent.const eq ==> Dependent.idR)
+             ==> (Dependent.idR ==> Dependent.idR ==> Dependent.idR)
+             ==> Dependent.idR
+             ==> (Dependent.idR ==> Dependent.idR ==> Dependent.idR)
+             ==> Tensor.eqfR
+             ==> Tensor.eqfR
+             ==> Tensor.eqfR
+             ==> Tensor.eqfR)
+          (@k r batch pos n_heads d_model d_head use_split_qkv_input).
     Proof. cbv [k]; repeat first [ t_step | apply einsum_input_Proper_dep ]. Qed.
 
-    #[export] Instance k_Proper {A r batch addA zeroA mulA defaultA pos n_heads d_model d_head use_split_qkv_input W_K b_K}
-      : Proper (Tensor.eqf ==> Tensor.eqf) (@k A r batch addA zeroA mulA defaultA pos n_heads d_model d_head use_split_qkv_input W_K b_K).
+    #[export] Instance k_Proper {A r batch pos n_heads d_model d_head use_split_qkv_input coerZ addA zeroA mulA W_K b_K}
+      : Proper (Tensor.eqf ==> Tensor.eqf) (@k A r batch pos n_heads d_model d_head use_split_qkv_input coerZ addA zeroA mulA W_K b_K).
     Proof. apply k_Proper_dep; repeat intro; subst; reflexivity. Qed.
 
     #[export] Instance v_Proper_dep {r batch pos n_heads d_model d_head use_split_qkv_input}
       : Dependent.Proper
-          ((Dependent.idR ==> Dependent.idR ==> Dependent.idR)
-             ==> Dependent.idR
+          ((Dependent.const eq ==> Dependent.idR)
              ==> (Dependent.idR ==> Dependent.idR ==> Dependent.idR)
              ==> Dependent.idR
+             ==> (Dependent.idR ==> Dependent.idR ==> Dependent.idR)
              ==> Tensor.eqfR
              ==> Tensor.eqfR
              ==> Tensor.eqfR
@@ -315,8 +314,8 @@ Module HookedTransformer.
           (@v r batch pos n_heads d_model d_head use_split_qkv_input).
     Proof. cbv [v]; repeat first [ t_step | apply einsum_input_Proper_dep ]. Qed.
 
-    #[export] Instance v_Proper {A r batch addA zeroA mulA defaultA pos n_heads d_model d_head use_split_qkv_input W_V b_V}
-      : Proper (Tensor.eqf ==> Tensor.eqf) (@v A r batch addA zeroA mulA defaultA pos n_heads d_model d_head use_split_qkv_input W_V b_V).
+    #[export] Instance v_Proper {A r batch pos n_heads d_model d_head use_split_qkv_input coerZ addA zeroA mulA W_V b_V}
+      : Proper (Tensor.eqf ==> Tensor.eqf) (@v A r batch pos n_heads d_model d_head use_split_qkv_input coerZ addA zeroA mulA W_V b_V).
     Proof. apply v_Proper_dep; repeat intro; subst; reflexivity. Qed.
 
     #[export] Instance attn_scores_Proper_dep {r batch pos n_heads d_model d_head use_split_qkv_input}
@@ -327,7 +326,6 @@ Module HookedTransformer.
              ==> Dependent.idR
              ==> (Dependent.idR ==> Dependent.idR ==> Dependent.idR)
              ==> (Dependent.idR ==> Dependent.idR ==> Dependent.idR)
-             ==> Dependent.idR
              ==> Tensor.eqfR
              ==> Tensor.eqfR
              ==> Tensor.eqfR
@@ -338,8 +336,8 @@ Module HookedTransformer.
           (@attn_scores r batch pos n_heads d_model d_head use_split_qkv_input).
     Proof. cbv [attn_scores]; repeat first [ t_step | apply q_Proper_dep | apply k_Proper_dep ]. Qed.
 
-    #[export] Instance attn_scores_Proper {r batch pos n_heads d_model d_head use_split_qkv_input A sqrtA coerZ addA zeroA mulA divA defaultA W_Q W_K b_Q b_K}
-      : Proper (Tensor.eqf ==> Tensor.eqf ==> Tensor.eqf) (@attn_scores r batch pos n_heads d_model d_head use_split_qkv_input A sqrtA coerZ addA zeroA mulA divA defaultA W_Q W_K b_Q b_K).
+    #[export] Instance attn_scores_Proper {r batch pos n_heads d_model d_head use_split_qkv_input A sqrtA coerZ addA zeroA mulA divA W_Q W_K b_Q b_K}
+      : Proper (Tensor.eqf ==> Tensor.eqf ==> Tensor.eqf) (@attn_scores r batch pos n_heads d_model d_head use_split_qkv_input A sqrtA coerZ addA zeroA mulA divA W_Q W_K b_Q b_K).
     Proof. apply attn_scores_Proper_dep; repeat intro; subst; reflexivity. Qed.
 
     #[export] Instance apply_causal_mask_Proper_dep {r batch pos n_heads n_ctx}
@@ -362,7 +360,6 @@ Module HookedTransformer.
              ==> Dependent.idR
              ==> (Dependent.idR ==> Dependent.idR ==> Dependent.idR)
              ==> (Dependent.idR ==> Dependent.idR ==> Dependent.idR)
-             ==> Dependent.idR
              ==> Tensor.eqfR
              ==> Tensor.eqfR
              ==> Tensor.eqfR
@@ -373,8 +370,8 @@ Module HookedTransformer.
           (@masked_attn_scores r batch pos n_heads d_model d_head n_ctx use_split_qkv_input).
     Proof. cbv [masked_attn_scores]; repeat first [ t_step | apply apply_causal_mask_Proper_dep | apply attn_scores_Proper_dep ]. Qed.
 
-    #[export] Instance masked_attn_scores_Proper {r batch pos n_heads d_model d_head n_ctx use_split_qkv_input A sqrtA coerZ addA zeroA mulA divA defaultA W_Q W_K b_Q b_K}
-      : Proper (Tensor.eqf ==> Tensor.eqf ==> Tensor.eqf) (@masked_attn_scores r batch pos n_heads d_model d_head n_ctx use_split_qkv_input A sqrtA coerZ addA zeroA mulA divA defaultA W_Q W_K b_Q b_K).
+    #[export] Instance masked_attn_scores_Proper {r batch pos n_heads d_model d_head n_ctx use_split_qkv_input A sqrtA coerZ addA zeroA mulA divA W_Q W_K b_Q b_K}
+      : Proper (Tensor.eqf ==> Tensor.eqf ==> Tensor.eqf) (@masked_attn_scores r batch pos n_heads d_model d_head n_ctx use_split_qkv_input A sqrtA coerZ addA zeroA mulA divA W_Q W_K b_Q b_K).
     Proof. apply masked_attn_scores_Proper_dep; repeat intro; subst; reflexivity. Qed.
 
     #[export] Instance pattern_Proper_dep {r batch pos n_heads d_model d_head n_ctx use_split_qkv_input}
@@ -386,7 +383,6 @@ Module HookedTransformer.
              ==> (Dependent.idR ==> Dependent.idR ==> Dependent.idR)
              ==> (Dependent.idR ==> Dependent.idR ==> Dependent.idR)
              ==> (Dependent.idR ==> Dependent.idR)
-             ==> Dependent.idR
              ==> Tensor.eqfR
              ==> Tensor.eqfR
              ==> Tensor.eqfR
@@ -397,8 +393,8 @@ Module HookedTransformer.
           (@pattern r batch pos n_heads d_model d_head n_ctx use_split_qkv_input).
     Proof. cbv [pattern]; repeat first [ t_step | apply masked_attn_scores_Proper_dep ]. Qed.
 
-    #[export] Instance pattern_Proper {r batch pos n_heads d_model d_head n_ctx use_split_qkv_input A sqrtA coerZ addA zeroA mulA divA expA defaultA W_Q W_K b_Q b_K}
-      : Proper (Tensor.eqf ==> Tensor.eqf ==> Tensor.eqf) (@pattern r batch pos n_heads d_model d_head n_ctx use_split_qkv_input A sqrtA coerZ addA zeroA mulA divA expA defaultA W_Q W_K b_Q b_K).
+    #[export] Instance pattern_Proper {r batch pos n_heads d_model d_head n_ctx use_split_qkv_input A sqrtA coerZ addA zeroA mulA divA expA W_Q W_K b_Q b_K}
+      : Proper (Tensor.eqf ==> Tensor.eqf ==> Tensor.eqf) (@pattern r batch pos n_heads d_model d_head n_ctx use_split_qkv_input A sqrtA coerZ addA zeroA mulA divA expA W_Q W_K b_Q b_K).
     Proof. apply pattern_Proper_dep; repeat intro; subst; reflexivity. Qed.
 
     #[export] Instance z_Proper_dep {r batch pos n_heads d_model d_head n_ctx use_split_qkv_input}
@@ -410,7 +406,6 @@ Module HookedTransformer.
              ==> (Dependent.idR ==> Dependent.idR ==> Dependent.idR)
              ==> (Dependent.idR ==> Dependent.idR ==> Dependent.idR)
              ==> (Dependent.idR ==> Dependent.idR)
-             ==> Dependent.idR
              ==> Tensor.eqfR
              ==> Tensor.eqfR
              ==> Tensor.eqfR
@@ -424,9 +419,9 @@ Module HookedTransformer.
           (@z r batch pos n_heads d_model d_head n_ctx use_split_qkv_input).
     Proof. cbv [z]; repeat first [ t_step | apply v_Proper_dep | apply pattern_Proper_dep ]. Qed.
 
-    #[export] Instance z_Proper {r batch pos n_heads d_model d_head n_ctx use_split_qkv_input A sqrtA coerZ addA zeroA mulA divA expA defaultA W_Q W_K W_V b_Q b_K b_V}
+    #[export] Instance z_Proper {r batch pos n_heads d_model d_head n_ctx use_split_qkv_input A sqrtA coerZ addA zeroA mulA divA expA W_Q W_K W_V b_Q b_K b_V}
       : Proper (Tensor.eqf ==> Tensor.eqf ==> Tensor.eqf ==> Tensor.eqf)
-        (@z r batch pos n_heads d_model d_head n_ctx use_split_qkv_input A sqrtA coerZ addA zeroA mulA divA expA defaultA W_Q W_K W_V b_Q b_K b_V).
+          (@z r batch pos n_heads d_model d_head n_ctx use_split_qkv_input A sqrtA coerZ addA zeroA mulA divA expA W_Q W_K W_V b_Q b_K b_V).
     Proof. apply z_Proper_dep; repeat intro; subst; reflexivity. Qed.
 
     #[export] Instance attn_out_Proper_dep {r batch pos n_heads d_model d_head n_ctx use_split_qkv_input}
@@ -438,7 +433,6 @@ Module HookedTransformer.
              ==> (Dependent.idR ==> Dependent.idR ==> Dependent.idR)
              ==> (Dependent.idR ==> Dependent.idR ==> Dependent.idR)
              ==> (Dependent.idR ==> Dependent.idR)
-             ==> Dependent.idR
              ==> Tensor.eqfR
              ==> Tensor.eqfR
              ==> Tensor.eqfR
@@ -454,9 +448,9 @@ Module HookedTransformer.
           (@attn_out r batch pos n_heads d_model d_head n_ctx use_split_qkv_input).
     Proof. cbv [attn_out]; repeat first [ t_step | apply z_Proper_dep ]. Qed.
 
-    #[export] Instance attn_out_Proper {r batch pos n_heads d_model d_head n_ctx use_split_qkv_input A sqrtA coerZ addA zeroA mulA divA expA defaultA W_Q W_K W_V W_O b_Q b_K b_V b_O}
+    #[export] Instance attn_out_Proper {r batch pos n_heads d_model d_head n_ctx use_split_qkv_input A sqrtA coerZ addA zeroA mulA divA expA W_Q W_K W_V W_O b_Q b_K b_V b_O}
       : Proper (Tensor.eqf ==> Tensor.eqf ==> Tensor.eqf ==> Tensor.eqf)
-          (@attn_out r batch pos n_heads d_model d_head n_ctx use_split_qkv_input A sqrtA coerZ addA zeroA mulA divA expA defaultA W_Q W_K W_V W_O b_Q b_K b_V b_O).
+          (@attn_out r batch pos n_heads d_model d_head n_ctx use_split_qkv_input A sqrtA coerZ addA zeroA mulA divA expA W_Q W_K W_V W_O b_Q b_K b_V b_O).
     Proof. apply attn_out_Proper_dep; repeat intro; subst; reflexivity. Qed.
   End Attention.
   Export (hints) Attention.
@@ -503,7 +497,6 @@ Module HookedTransformer.
              ==> (Dependent.idR ==> Dependent.idR ==> Dependent.idR)
              ==> (Dependent.idR ==> Dependent.idR)
              ==> Dependent.idR
-             ==> Dependent.idR
              ==> match normalization_type return Dependent.relation (fun A => match normalization_type with Some LN => _ | None => _ end) with
              | Some LN => Tensor.eqfR (s:=[d_model])
              | None => Dependent.const eq
@@ -517,8 +510,8 @@ Module HookedTransformer.
           (@ln1 r batch pos n_heads d_model use_split_qkv_input normalization_type).
     Proof. cbv [ln1]; repeat first [ t_step | apply LayerNorm.forward_Proper_dep ]. Qed.
 
-    #[export] Instance ln1_Proper {r batch pos n_heads d_model use_split_kqv_input normalization_type A zeroA coerZ addA subA mulA divA sqrtA default eps ln1_w ln1_b}
-      : Proper (Tensor.eqf ==> Tensor.eqf) (@ln1 r batch pos n_heads d_model use_split_kqv_input normalization_type A zeroA coerZ addA subA mulA divA sqrtA default eps ln1_w ln1_b).
+    #[export] Instance ln1_Proper {r batch pos n_heads d_model use_split_kqv_input normalization_type A zeroA coerZ addA subA mulA divA sqrtA eps ln1_w ln1_b}
+      : Proper (Tensor.eqf ==> Tensor.eqf) (@ln1 r batch pos n_heads d_model use_split_kqv_input normalization_type A zeroA coerZ addA subA mulA divA sqrtA eps ln1_w ln1_b).
     Proof. apply ln1_Proper_dep; repeat intro; subst; break_innermost_match; reflexivity. Qed.
 
     #[export] Instance ln2_Proper_dep {r batch pos n_heads d_model use_split_qkv_input normalization_type}
@@ -530,7 +523,6 @@ Module HookedTransformer.
              ==> (Dependent.idR ==> Dependent.idR ==> Dependent.idR)
              ==> (Dependent.idR ==> Dependent.idR ==> Dependent.idR)
              ==> (Dependent.idR ==> Dependent.idR)
-             ==> Dependent.idR
              ==> Dependent.idR
              ==> match normalization_type return Dependent.relation (fun A => match normalization_type with Some LN => _ | None => _ end) with
              | Some LN => Tensor.eqfR (s:=[d_model])
@@ -545,8 +537,8 @@ Module HookedTransformer.
           (@ln2 r batch pos n_heads d_model use_split_qkv_input normalization_type).
     Proof. cbv [ln2]; repeat first [ t_step | apply LayerNorm.forward_Proper_dep ]. Qed.
 
-    #[export] Instance ln2_Proper {r batch pos n_heads d_model use_split_kqv_input normalization_type A zeroA coerZ addA subA mulA divA sqrtA default eps ln2_w ln2_b}
-      : Proper (Tensor.eqf ==> Tensor.eqf) (@ln2 r batch pos n_heads d_model use_split_kqv_input normalization_type A zeroA coerZ addA subA mulA divA sqrtA default eps ln2_w ln2_b).
+    #[export] Instance ln2_Proper {r batch pos n_heads d_model use_split_kqv_input normalization_type A zeroA coerZ addA subA mulA divA sqrtA eps ln2_w ln2_b}
+      : Proper (Tensor.eqf ==> Tensor.eqf) (@ln2 r batch pos n_heads d_model use_split_kqv_input normalization_type A zeroA coerZ addA subA mulA divA sqrtA eps ln2_w ln2_b).
     Proof. apply ln2_Proper_dep; repeat intro; subst; break_innermost_match; reflexivity. Qed.
 
     #[export] Instance attn_only_out_Proper_dep {r batch pos n_heads d_model d_head n_ctx use_split_qkv_input normalization_type}
@@ -559,7 +551,6 @@ Module HookedTransformer.
              ==> (Dependent.idR ==> Dependent.idR ==> Dependent.idR)
              ==> (Dependent.idR ==> Dependent.idR)
              ==> (Dependent.idR ==> Dependent.idR)
-             ==> Dependent.idR
              ==> Tensor.eqfR
              ==> Tensor.eqfR
              ==> Tensor.eqfR
@@ -587,8 +578,8 @@ Module HookedTransformer.
       all: first [ apply query_input_Proper_dep | apply key_input_Proper_dep | apply value_input_Proper_dep ]; t.
     Qed.
 
-    #[export] Instance attn_only_out_Proper {r batch pos n_heads d_model d_head n_ctx use_split_kqv_input normalization_type A zeroA coerZ addA subA mulA divA sqrtA expA default W_Q W_K W_V W_O b_Q b_K b_V b_O eps ln1_w ln1_b}
-      : Proper (Tensor.eqf ==> Tensor.eqf) (@attn_only_out r batch pos n_heads d_model d_head n_ctx use_split_kqv_input normalization_type A zeroA coerZ addA subA mulA divA sqrtA expA default W_Q W_K W_V W_O b_Q b_K b_V b_O eps ln1_w ln1_b).
+    #[export] Instance attn_only_out_Proper {r batch pos n_heads d_model d_head n_ctx use_split_kqv_input normalization_type A zeroA coerZ addA subA mulA divA sqrtA expA W_Q W_K W_V W_O b_Q b_K b_V b_O eps ln1_w ln1_b}
+      : Proper (Tensor.eqf ==> Tensor.eqf) (@attn_only_out r batch pos n_heads d_model d_head n_ctx use_split_kqv_input normalization_type A zeroA coerZ addA subA mulA divA sqrtA expA W_Q W_K W_V W_O b_Q b_K b_V b_O eps ln1_w ln1_b).
     Proof. apply attn_only_out_Proper_dep; repeat intro; subst; break_innermost_match; reflexivity. Qed.
 
     #[export] Instance attn_masked_attn_scores_Proper_dep {r batch pos n_heads d_model d_head n_ctx use_split_qkv_input normalization_type}
@@ -600,7 +591,6 @@ Module HookedTransformer.
              ==> (Dependent.idR ==> Dependent.idR ==> Dependent.idR)
              ==> (Dependent.idR ==> Dependent.idR ==> Dependent.idR)
              ==> (Dependent.idR ==> Dependent.idR)
-             ==> Dependent.idR
              ==> Tensor.eqfR
              ==> Tensor.eqfR
              ==> Tensor.eqfR
@@ -624,8 +614,8 @@ Module HookedTransformer.
       all: first [ apply query_input_Proper_dep | apply key_input_Proper_dep ]; t.
     Qed.
 
-    #[export] Instance attn_masked_attn_scores_Proper {r batch pos n_heads d_model d_head n_ctx use_split_kqv_input normalization_type A zeroA coerZ addA subA mulA divA sqrtA default W_Q W_K b_Q b_K eps ln1_w ln1_b}
-      : Proper (Tensor.eqf ==> Tensor.eqf) (@HookedTransformer.TransformerBlock.attn_masked_attn_scores r batch pos n_heads d_model d_head n_ctx use_split_kqv_input normalization_type A zeroA coerZ addA subA mulA divA sqrtA default W_Q W_K b_Q b_K eps ln1_w ln1_b).
+    #[export] Instance attn_masked_attn_scores_Proper {r batch pos n_heads d_model d_head n_ctx use_split_kqv_input normalization_type A zeroA coerZ addA subA mulA divA sqrtA W_Q W_K b_Q b_K eps ln1_w ln1_b}
+      : Proper (Tensor.eqf ==> Tensor.eqf) (@HookedTransformer.TransformerBlock.attn_masked_attn_scores r batch pos n_heads d_model d_head n_ctx use_split_kqv_input normalization_type A zeroA coerZ addA subA mulA divA sqrtA W_Q W_K b_Q b_K eps ln1_w ln1_b).
     Proof. apply attn_masked_attn_scores_Proper_dep; repeat intro; subst; break_innermost_match; reflexivity. Qed.
 
     #[export] Instance attn_pattern_Proper_dep {r batch pos n_heads d_model d_head n_ctx use_split_qkv_input normalization_type}
@@ -638,7 +628,6 @@ Module HookedTransformer.
              ==> (Dependent.idR ==> Dependent.idR ==> Dependent.idR)
              ==> (Dependent.idR ==> Dependent.idR)
              ==> (Dependent.idR ==> Dependent.idR)
-             ==> Dependent.idR
              ==> Tensor.eqfR
              ==> Tensor.eqfR
              ==> Tensor.eqfR
@@ -662,8 +651,8 @@ Module HookedTransformer.
       all: first [ apply query_input_Proper_dep | apply key_input_Proper_dep ]; t.
     Qed.
 
-    #[export] Instance attn_pattern_Proper {r batch pos n_heads d_model d_head n_ctx use_split_kqv_input normalization_type A zeroA coerZ addA subA mulA divA sqrtA expA default W_Q W_K b_Q b_K eps ln1_w ln1_b}
-      : Proper (Tensor.eqf ==> Tensor.eqf) (@HookedTransformer.TransformerBlock.attn_pattern r batch pos n_heads d_model d_head n_ctx use_split_kqv_input normalization_type A zeroA coerZ addA subA mulA divA sqrtA expA default W_Q W_K b_Q b_K eps ln1_w ln1_b).
+    #[export] Instance attn_pattern_Proper {r batch pos n_heads d_model d_head n_ctx use_split_kqv_input normalization_type A zeroA coerZ addA subA mulA divA sqrtA expA W_Q W_K b_Q b_K eps ln1_w ln1_b}
+      : Proper (Tensor.eqf ==> Tensor.eqf) (@HookedTransformer.TransformerBlock.attn_pattern r batch pos n_heads d_model d_head n_ctx use_split_kqv_input normalization_type A zeroA coerZ addA subA mulA divA sqrtA expA W_Q W_K b_Q b_K eps ln1_w ln1_b).
     Proof. apply attn_pattern_Proper_dep; repeat intro; subst; break_innermost_match; reflexivity. Qed.
   End TransformerBlock.
   Export (hints) TransformerBlock.
@@ -691,15 +680,15 @@ Module HookedTransformer.
 
     #[export] Instance resid_postembed_Proper_dep {d_vocab d_model n_ctx r batch pos}
       : Dependent.Proper
-          ((Dependent.idR ==> Dependent.idR ==> Dependent.idR)
-             ==> Dependent.idR
+          ((Dependent.const eq ==> Dependent.idR)
+             ==> (Dependent.idR ==> Dependent.idR ==> Dependent.idR)
              ==> Tensor.eqfR ==> Tensor.eqfR
              ==> Dependent.const Tensor.eqf ==> Tensor.eqfR)
           (@resid_postembed d_vocab d_model n_ctx r batch pos).
     Proof. cbv [resid_postembed]; t; first [ apply embed_Proper_dep | apply pos_embed_Proper_dep ]; t. Qed.
 
-    #[export] Instance resid_postembed_Proper {d_vocab d_model n_ctx r batch pos A addA default W_E W_pos}
-      : Proper (Tensor.eqf ==> Tensor.eqf) (@resid_postembed d_vocab d_model n_ctx r batch pos A addA default W_E W_pos).
+    #[export] Instance resid_postembed_Proper {d_vocab d_model n_ctx r batch pos A coerZ addA W_E W_pos}
+      : Proper (Tensor.eqf ==> Tensor.eqf) (@resid_postembed d_vocab d_model n_ctx r batch pos A coerZ addA W_E W_pos).
     Proof. apply resid_postembed_Proper_dep; repeat intro; subst; reflexivity. Qed.
 
     #[export] Polymorphic Instance blocks_Proper_dep {n_heads d_model d_head n_ctx r batch pos normalization_type}
@@ -712,7 +701,6 @@ Module HookedTransformer.
              ==> (Dependent.idR ==> Dependent.idR ==> Dependent.idR)
              ==> (Dependent.idR ==> Dependent.idR)
              ==> (Dependent.idR ==> Dependent.idR)
-             ==> Dependent.idR
              ==> Dependent.idR
              ==> List.Forall2 ∘ (Tensor.eqfR * Tensor.eqfR
                                  * Tensor.eqfR * Tensor.eqfR
@@ -737,8 +725,8 @@ Module HookedTransformer.
       apply TransformerBlock.attn_only_out_Proper_dep; t.
     Qed.
 
-    #[export] Polymorphic Instance blocks_Proper {n_heads d_model d_head n_ctx r batch pos normalization_type A zeroA coerZ addA subA mulA divA sqrtA expA default eps blocks_params}
-      : Proper (List.Forall2 (Tensor.eqf ==> Tensor.eqf))%signature (@blocks n_heads d_model d_head n_ctx r batch pos normalization_type A zeroA coerZ addA subA mulA divA sqrtA expA default eps blocks_params).
+    #[export] Polymorphic Instance blocks_Proper {n_heads d_model d_head n_ctx r batch pos normalization_type A zeroA coerZ addA subA mulA divA sqrtA expA eps blocks_params}
+      : Proper (List.Forall2 (Tensor.eqf ==> Tensor.eqf))%signature (@blocks n_heads d_model d_head n_ctx r batch pos normalization_type A zeroA coerZ addA subA mulA divA sqrtA expA eps blocks_params).
     Proof. apply blocks_Proper_dep; repeat intro; subst; break_innermost_match; reflexivity. Qed.
 
     #[export] Instance ln_final_Proper_dep {d_model r batch pos normalization_type}
@@ -750,7 +738,6 @@ Module HookedTransformer.
              ==> (Dependent.idR ==> Dependent.idR ==> Dependent.idR)
              ==> (Dependent.idR ==> Dependent.idR ==> Dependent.idR)
              ==> (Dependent.idR ==> Dependent.idR)
-             ==> Dependent.idR
              ==> Dependent.idR
              ==> match normalization_type return Dependent.relation (fun A => match normalization_type with Some LN => _ | None => _ end) with
              | Some LN => Tensor.eqfR (s:=[d_model])
@@ -765,8 +752,8 @@ Module HookedTransformer.
           (@ln_final d_model r batch pos normalization_type).
     Proof. cbv [ln_final]; repeat first [ t_step | apply LayerNorm.forward_Proper_dep ]. Qed.
 
-    #[export] Instance ln_final_Proper {d_model r batch pos normalization_type A zeroA coerZ addA subA mulA divA sqrtA default eps ln_final_w ln_final_b}
-      : Proper (Tensor.eqf ==> Tensor.eqf) (@ln_final d_model r batch pos normalization_type A zeroA coerZ addA subA mulA divA sqrtA default eps ln_final_w ln_final_b).
+    #[export] Instance ln_final_Proper {d_model r batch pos normalization_type A zeroA coerZ addA subA mulA divA sqrtA eps ln_final_w ln_final_b}
+      : Proper (Tensor.eqf ==> Tensor.eqf) (@ln_final d_model r batch pos normalization_type A zeroA coerZ addA subA mulA divA sqrtA eps ln_final_w ln_final_b).
     Proof. apply ln_final_Proper_dep; repeat intro; subst; break_innermost_match; reflexivity. Qed.
 
     #[export] Instance unembed_Proper_dep {d_vocab_out d_model r batch pos}
@@ -787,7 +774,7 @@ Module HookedTransformer.
 
     #[export] Instance blocks_cps_Proper_dep {n_heads d_model d_head n_ctx r batch pos normalization_type}
       : Dependent.Proper
-                           (Dependent.idR
+          (Dependent.idR
              ==> (Dependent.const eq ==> Dependent.idR)
              ==> (Dependent.idR ==> Dependent.idR ==> Dependent.idR)
              ==> (Dependent.idR ==> Dependent.idR ==> Dependent.idR)
@@ -795,7 +782,6 @@ Module HookedTransformer.
              ==> (Dependent.idR ==> Dependent.idR ==> Dependent.idR)
              ==> (Dependent.idR ==> Dependent.idR)
              ==> (Dependent.idR ==> Dependent.idR)
-             ==> Dependent.idR
              ==> Dependent.idR
              ==> List.Forall2 ∘ (Tensor.eqfR * Tensor.eqfR
                                  * Tensor.eqfR * Tensor.eqfR
@@ -814,7 +800,7 @@ Module HookedTransformer.
                 ==> Dependent.lift2_1 Tensor.eqfR
                 ==> (Dependent.lift2_1 Tensor.eqfR ==> Dependent.lift2_2 Dependent.idR)
                 ==> Dependent.lift2_2 Dependent.idR))
-                           (@blocks_cps n_heads d_model d_head n_ctx r batch pos normalization_type).
+          (@blocks_cps n_heads d_model d_head n_ctx r batch pos normalization_type).
     Proof.
       cbv [Dependent.Proper Dependent.respectful blocks_cps with_default Dependent.forall_relation Dependent.respectful2]; clear.
       repeat first [ lazymatch goal with H : Forall2 _ _ _ |- _ => fail 1 end | intro ].
@@ -829,13 +815,13 @@ Module HookedTransformer.
       let IH := multimatch goal with H : _ |- _ => H end in
       apply IH; clear IH; repeat intro; eauto; [].
       break_innermost_match.
-      apply Tensor.PArray.checkpoint_Proper_dep; try assumption; [].
+      apply Tensor.PArray.checkpoint_Proper_dep; try assumption; auto; [].
       apply TransformerBlock.attn_only_out_Proper_dep; t.
     Qed.
 
-    #[export] Instance blocks_cps_Proper {n_heads d_model d_head n_ctx r batch pos normalization_type A zeroA coerZ addA subA mulA divA sqrtA expA default eps blocks_params T R}
+    #[export] Instance blocks_cps_Proper {n_heads d_model d_head n_ctx r batch pos normalization_type A zeroA coerZ addA subA mulA divA sqrtA expA eps blocks_params T R}
       : Proper (eq ==> Tensor.eqf ==> (Tensor.eqf ==> R) ==> R)
-          (@blocks_cps n_heads d_model d_head n_ctx r batch pos normalization_type A zeroA coerZ addA subA mulA divA sqrtA expA default eps blocks_params T).
+          (@blocks_cps n_heads d_model d_head n_ctx r batch pos normalization_type A zeroA coerZ addA subA mulA divA sqrtA expA eps blocks_params T).
     Proof. apply blocks_cps_Proper_dep; repeat intro; subst; break_innermost_match; reflexivity. Qed.
 
     #[export] Instance logits_Proper_dep {d_vocab d_vocab_out n_heads d_model d_head n_ctx r batch pos normalization_type}
@@ -848,7 +834,6 @@ Module HookedTransformer.
              ==> (Dependent.idR ==> Dependent.idR ==> Dependent.idR)
              ==> (Dependent.idR ==> Dependent.idR)
              ==> (Dependent.idR ==> Dependent.idR)
-             ==> Dependent.idR
              ==> Dependent.idR
              ==> Tensor.eqfR
              ==> Tensor.eqfR
@@ -889,9 +874,9 @@ Module HookedTransformer.
       all: first [ apply resid_postembed_Proper_dep | apply embed_Proper_dep | apply pos_embed_Proper_dep | apply ln_final_Proper_dep | apply unembed_Proper_dep ]; t.
     Qed.
 
-    #[export] Instance logits_Proper {d_vocab d_vocab_out n_heads d_model d_head n_ctx r batch pos normalization_type A zeroA coerZ addA subA mulA divA sqrtA expA default eps W_E W_pos blocks_params ln_final_w ln_final_b W_U b_U}
+    #[export] Instance logits_Proper {d_vocab d_vocab_out n_heads d_model d_head n_ctx r batch pos normalization_type A zeroA coerZ addA subA mulA divA sqrtA expA eps W_E W_pos blocks_params ln_final_w ln_final_b W_U b_U}
       : Proper (Tensor.eqf ==> Tensor.eqf)
-          (@logits d_vocab d_vocab_out n_heads d_model d_head n_ctx r batch pos normalization_type A zeroA coerZ addA subA mulA divA sqrtA expA default eps W_E W_pos blocks_params ln_final_w ln_final_b W_U b_U).
+          (@logits d_vocab d_vocab_out n_heads d_model d_head n_ctx r batch pos normalization_type A zeroA coerZ addA subA mulA divA sqrtA expA eps W_E W_pos blocks_params ln_final_w ln_final_b W_U b_U).
     Proof. apply logits_Proper_dep; repeat intro; subst; break_innermost_match; reflexivity. Qed.
 
     #[export] Instance forward_Proper_dep {d_vocab d_vocab_out n_heads d_model d_head n_ctx r batch pos normalization_type}
@@ -904,7 +889,6 @@ Module HookedTransformer.
              ==> (Dependent.idR ==> Dependent.idR ==> Dependent.idR)
              ==> (Dependent.idR ==> Dependent.idR)
              ==> (Dependent.idR ==> Dependent.idR)
-             ==> Dependent.idR
              ==> Dependent.idR
              ==> Tensor.eqfR
              ==> Tensor.eqfR
@@ -935,9 +919,9 @@ Module HookedTransformer.
           (@forward d_vocab d_vocab_out n_heads d_model d_head n_ctx r batch pos normalization_type)
       := _.
 
-    #[export] Instance forward_Proper {d_vocab d_vocab_out n_heads d_model d_head n_ctx r batch pos normalization_type A zeroA coerZ addA subA mulA divA sqrtA expA default eps W_E W_pos blocks_params ln_final_w ln_final_b W_U b_U}
+    #[export] Instance forward_Proper {d_vocab d_vocab_out n_heads d_model d_head n_ctx r batch pos normalization_type A zeroA coerZ addA subA mulA divA sqrtA expA eps W_E W_pos blocks_params ln_final_w ln_final_b W_U b_U}
       : Proper (Tensor.eqf ==> Tensor.eqf)
-          (@forward d_vocab d_vocab_out n_heads d_model d_head n_ctx r batch pos normalization_type A zeroA coerZ addA subA mulA divA sqrtA expA default eps W_E W_pos blocks_params ln_final_w ln_final_b W_U b_U)
+          (@forward d_vocab d_vocab_out n_heads d_model d_head n_ctx r batch pos normalization_type A zeroA coerZ addA subA mulA divA sqrtA expA eps W_E W_pos blocks_params ln_final_w ln_final_b W_U b_U)
       := _.
 
     #[export] Instance blocks_attn_masked_attn_scores_Proper_dep {n_heads d_model d_head n_ctx r batch pos normalization_type}
@@ -949,7 +933,6 @@ Module HookedTransformer.
              ==> (Dependent.idR ==> Dependent.idR ==> Dependent.idR)
              ==> (Dependent.idR ==> Dependent.idR ==> Dependent.idR)
              ==> (Dependent.idR ==> Dependent.idR)
-             ==> Dependent.idR
              ==> Dependent.idR
              ==> List.Forall2 ∘ (Tensor.eqfR * Tensor.eqfR
                                  * Tensor.eqfR * Tensor.eqfR
@@ -974,9 +957,9 @@ Module HookedTransformer.
       apply TransformerBlock.attn_masked_attn_scores_Proper_dep; t.
     Qed.
 
-    #[export] Instance blocks_attn_masked_attn_scores_Proper {n_heads d_model d_head n_ctx r batch pos normalization_type A zeroA coerZ addA subA mulA divA sqrtA default eps blocks_params}
+    #[export] Instance blocks_attn_masked_attn_scores_Proper {n_heads d_model d_head n_ctx r batch pos normalization_type A zeroA coerZ addA subA mulA divA sqrtA eps blocks_params}
       : Proper (List.Forall2 (Tensor.eqf ==> Tensor.eqf))%signature
-          (@HookedTransformer.HookedTransformer.blocks_attn_masked_attn_scores n_heads d_model d_head n_ctx r batch pos normalization_type A zeroA coerZ addA subA mulA divA sqrtA default eps blocks_params).
+          (@HookedTransformer.HookedTransformer.blocks_attn_masked_attn_scores n_heads d_model d_head n_ctx r batch pos normalization_type A zeroA coerZ addA subA mulA divA sqrtA eps blocks_params).
     Proof. apply blocks_attn_masked_attn_scores_Proper_dep; repeat intro; subst; break_innermost_match; reflexivity. Qed.
 
     #[export] Instance blocks_attn_pattern_Proper_dep {n_heads d_model d_head n_ctx r batch pos normalization_type}
@@ -989,7 +972,6 @@ Module HookedTransformer.
              ==> (Dependent.idR ==> Dependent.idR ==> Dependent.idR)
              ==> (Dependent.idR ==> Dependent.idR)
              ==> (Dependent.idR ==> Dependent.idR)
-             ==> Dependent.idR
              ==> Dependent.idR
              ==> List.Forall2 ∘ (Tensor.eqfR * Tensor.eqfR
                                  * Tensor.eqfR * Tensor.eqfR
@@ -1014,9 +996,9 @@ Module HookedTransformer.
       apply TransformerBlock.attn_pattern_Proper_dep; t.
     Qed.
 
-    #[export] Instance blocks_attn_pattern_Proper {n_heads d_model d_head n_ctx r batch pos normalization_type A zeroA coerZ addA subA mulA divA sqrtA expA default eps blocks_params}
+    #[export] Instance blocks_attn_pattern_Proper {n_heads d_model d_head n_ctx r batch pos normalization_type A zeroA coerZ addA subA mulA divA sqrtA expA eps blocks_params}
       : Proper (List.Forall2 (Tensor.eqf ==> Tensor.eqf))%signature
-          (@HookedTransformer.HookedTransformer.blocks_attn_pattern n_heads d_model d_head n_ctx r batch pos normalization_type A zeroA coerZ addA subA mulA divA sqrtA expA default eps blocks_params).
+          (@HookedTransformer.HookedTransformer.blocks_attn_pattern n_heads d_model d_head n_ctx r batch pos normalization_type A zeroA coerZ addA subA mulA divA sqrtA expA eps blocks_params).
     Proof. apply blocks_attn_pattern_Proper_dep; repeat intro; subst; break_innermost_match; reflexivity. Qed.
 
     #[export] Instance masked_attn_scores_Proper_dep {d_vocab n_heads d_model d_head n_ctx r batch pos normalization_type}
@@ -1029,7 +1011,6 @@ Module HookedTransformer.
              ==> (Dependent.idR ==> Dependent.idR ==> Dependent.idR)
              ==> (Dependent.idR ==> Dependent.idR)
              ==> (Dependent.idR ==> Dependent.idR)
-             ==> Dependent.idR
              ==> Dependent.idR
              ==> Tensor.eqfR
              ==> Tensor.eqfR
@@ -1059,7 +1040,7 @@ Module HookedTransformer.
                   (epose proof (List.nth_error_Proper_dep_Forall2
                                   _ _ _
                                   xs ys
-                                  (blocks_attn_masked_attn_scores_Proper_dep _ _ _ _ _ _ _ _ _ _ _ _ _ _ _ _)
+                                  (blocks_attn_masked_attn_scores_Proper_dep _ _ _ _ _ _ _ _ _ _ _ _ _)
                                   n n eq_refl) as H';
                    rewrite Hx, Hy in H'; cbv [option_eq] in H'; clear Hx Hy;
                    try now exfalso);
@@ -1075,9 +1056,9 @@ Module HookedTransformer.
       all: first [ apply resid_postembed_Proper_dep | apply embed_Proper_dep | apply pos_embed_Proper_dep | apply ln_final_Proper_dep | apply unembed_Proper_dep ]; t.
     Qed.
 
-    #[export] Instance masked_attn_scores_Proper {d_vocab n_heads d_model d_head n_ctx r batch pos normalization_type A zeroA coerZ addA subA mulA divA sqrtA expA default eps W_E W_pos blocks_params}
+    #[export] Instance masked_attn_scores_Proper {d_vocab n_heads d_model d_head n_ctx r batch pos normalization_type A zeroA coerZ addA subA mulA divA sqrtA expA eps W_E W_pos blocks_params}
       : Proper (eq ==> Tensor.eqf ==> option_eq Tensor.eqf)
-          (@HookedTransformer.HookedTransformer.masked_attn_scores d_vocab n_heads d_model d_head n_ctx r batch pos normalization_type A zeroA coerZ addA subA mulA divA sqrtA expA default eps W_E W_pos blocks_params).
+          (@HookedTransformer.HookedTransformer.masked_attn_scores d_vocab n_heads d_model d_head n_ctx r batch pos normalization_type A zeroA coerZ addA subA mulA divA sqrtA expA eps W_E W_pos blocks_params).
     Proof. apply masked_attn_scores_Proper_dep; repeat intro; subst; break_innermost_match; reflexivity. Qed.
 
     #[export] Instance attn_pattern_Proper_dep {d_vocab n_heads d_model d_head n_ctx r batch pos normalization_type}
@@ -1090,7 +1071,6 @@ Module HookedTransformer.
              ==> (Dependent.idR ==> Dependent.idR ==> Dependent.idR)
              ==> (Dependent.idR ==> Dependent.idR)
              ==> (Dependent.idR ==> Dependent.idR)
-             ==> Dependent.idR
              ==> Dependent.idR
              ==> Tensor.eqfR
              ==> Tensor.eqfR
@@ -1120,7 +1100,7 @@ Module HookedTransformer.
                   (epose proof (List.nth_error_Proper_dep_Forall2
                                   _ _ _
                                   xs ys
-                                  (blocks_attn_pattern_Proper_dep _ _ _ _ _ _ _ _ _ _ _ _ _ _ _ _ _)
+                                  (blocks_attn_pattern_Proper_dep _ _ _ _ _ _ _ _ _ _ _ _ _ _)
                                   n n eq_refl) as H';
                    rewrite Hx, Hy in H'; cbv [option_eq] in H'; clear Hx Hy;
                    try now exfalso);
@@ -1135,9 +1115,9 @@ Module HookedTransformer.
       all: first [ apply resid_postembed_Proper_dep | apply embed_Proper_dep | apply pos_embed_Proper_dep | apply ln_final_Proper_dep | apply unembed_Proper_dep ]; t.
     Qed.
 
-    #[export] Instance attn_pattern_Proper {d_vocab n_heads d_model d_head n_ctx r batch pos normalization_type A zeroA coerZ addA subA mulA divA sqrtA expA default eps W_E W_pos blocks_params}
+    #[export] Instance attn_pattern_Proper {d_vocab n_heads d_model d_head n_ctx r batch pos normalization_type A zeroA coerZ addA subA mulA divA sqrtA expA eps W_E W_pos blocks_params}
       : Proper (eq ==> Tensor.eqf ==> option_eq Tensor.eqf)
-          (@HookedTransformer.HookedTransformer.attn_pattern d_vocab n_heads d_model d_head n_ctx r batch pos normalization_type A zeroA coerZ addA subA mulA divA sqrtA expA default eps W_E W_pos blocks_params).
+          (@HookedTransformer.HookedTransformer.attn_pattern d_vocab n_heads d_model d_head n_ctx r batch pos normalization_type A zeroA coerZ addA subA mulA divA sqrtA expA eps W_E W_pos blocks_params).
     Proof. apply attn_pattern_Proper_dep; repeat intro; subst; break_innermost_match; reflexivity. Qed.
   End HookedTransformer.
   Export (hints) HookedTransformer.
